check

DenotSem/Consistency.thy
@@ -1,48 +1,48 @@
 theory Consistency
-  imports LaurentValues
+  imports IntersectionTypes
 begin
 
 section "Consistency"
 
-fun consistent :: "val \<Rightarrow> val \<Rightarrow> bool" (infix "~" 52) where
-  "(VNat n) ~ (VNat m) = (n = m)" |
-  "(v1\<mapsto>v1') ~ (VNat m) = False" |
-  "(VNat n) ~ (v2\<mapsto>v2') = False" | 
-  "(v1\<mapsto>v1') ~ (v2\<mapsto>v2') = ((v1 ~ v2 \<and> v1' ~ v2') \<or> \<not> (v1 ~ v2))" |
-  "(VNat n) ~ (v2 \<squnion> v2') = (VNat n ~ v2 \<and> VNat n ~ v2')" |
-  "(v1\<mapsto>v1') ~ (v2 \<squnion> v2') = ((v1\<mapsto>v1') ~ v2 \<and> (v1\<mapsto>v1') ~ v2')" |
-  "(v1\<squnion>v1') ~ v2 = (v1 ~ v2 \<and> v1' ~ v2)" 
+fun consistent :: "ty \<Rightarrow> ty \<Rightarrow> bool" (infix "~" 52) where
+  "(TNat n) ~ (TNat m) = (n = m)" |
+  "(v1\<rightarrow>v1') ~ (TNat m) = False" |
+  "(TNat n) ~ (v2\<rightarrow>v2') = False" | 
+  "(v1\<rightarrow>v1') ~ (v2\<rightarrow>v2') = ((v1 ~ v2 \<and> v1' ~ v2') \<or> \<not> (v1 ~ v2))" |
+  "(TNat n) ~ (v2 \<sqinter> v2') = (TNat n ~ v2 \<and> TNat n ~ v2')" |
+  "(v1\<rightarrow>v1') ~ (v2 \<sqinter> v2') = ((v1\<rightarrow>v1') ~ v2 \<and> (v1\<rightarrow>v1') ~ v2')" |
+  "(v1\<sqinter>v1') ~ v2 = (v1 ~ v2 \<and> v1' ~ v2)" 
   
-(*fun consis_env :: "val list \<Rightarrow> val list \<Rightarrow> bool" where
+(*fun consis_env :: "ty list \<Rightarrow> ty list \<Rightarrow> bool" where
   "consis_env [] [] = True" |
   "consis_env [] (v'#\<rho>') = False" | 
   "consis_env (v#\<rho>) [] = False" |
   "consis_env (v#\<rho>) (v'#\<rho>') = (v ~ v' \<and> consis_env \<rho> \<rho>')"
 *)
-abbreviation consis_env :: "val list \<Rightarrow> val list \<Rightarrow> bool" where
+abbreviation consis_env :: "ty list \<Rightarrow> ty list \<Rightarrow> bool" where
   "consis_env \<rho> \<rho>' \<equiv> length \<rho> = length \<rho>' \<and> (\<forall> k. k < length \<rho> \<longrightarrow> \<rho>!k ~ \<rho>'!k)"
   
-fun is_val :: "val \<Rightarrow> bool" where
-  "is_val (VNat n) = True" |
-  "is_val (v \<mapsto> v') = (is_val v \<and> is_val v')" |
-  "is_val (v1 \<squnion> v2) = (is_val v1 \<and> is_val v2 \<and> v1 ~ v2)"
+fun is_val :: "ty \<Rightarrow> bool" where
+  "is_val (TNat n) = True" |
+  "is_val (v \<rightarrow> v') = (is_val v \<and> is_val v')" |
+  "is_val (v1 \<sqinter> v2) = (is_val v1 \<and> is_val v2 \<and> v1 ~ v2)"
 
-abbreviation val_env :: "val list \<Rightarrow> bool" where
+abbreviation val_env :: "ty list \<Rightarrow> bool" where
   "val_env \<rho> \<equiv> \<forall>k. k < length \<rho> \<longrightarrow> is_val (\<rho>!k)"
 
-abbreviation env_le :: "val list \<Rightarrow> val list \<Rightarrow> bool" (infix "\<sqsubseteq>" 52) where 
-  "(\<rho>::val list) \<sqsubseteq> \<rho>' \<equiv> length \<rho> = length \<rho>' \<and> (\<forall> k. k < length \<rho>  \<longrightarrow> \<rho>!k \<sqsubseteq> \<rho>'!k)" 
- 
-lemma consis_join_R[intro!]: "\<lbrakk> v1 ~ v2; v1 ~ v3 \<rbrakk> \<Longrightarrow> v1 ~ v2 \<squnion> v3"
+abbreviation env_le :: "ty list \<Rightarrow> ty list \<Rightarrow> bool" (infix "<:" 52) where 
+  "(\<rho>::ty list) <: \<rho>' \<equiv> length \<rho> = length \<rho>' \<and> (\<forall> k. k < length \<rho>  \<longrightarrow> \<rho>!k <: \<rho>'!k)" 
+
+lemma consis_join_R[intro!]: "\<lbrakk> v1 ~ v2; v1 ~ v3 \<rbrakk> \<Longrightarrow> v1 ~ v2 \<sqinter> v3"
   by (induction v1) auto
 
-lemma consis_join_L[intro!]: "\<lbrakk> v1 ~ v3; v2 ~ v3 \<rbrakk> \<Longrightarrow> v1 \<squnion> v2 ~ v3"
+lemma consis_join_L[intro!]: "\<lbrakk> v1 ~ v3; v2 ~ v3 \<rbrakk> \<Longrightarrow> v1 \<sqinter> v2 ~ v3"
   by auto  
   
-lemma consis_join_L_inv[elim!]: "\<lbrakk> v1\<squnion>v2 ~ v; \<lbrakk> v1 ~ v; v2 ~ v \<rbrakk> \<Longrightarrow> P \<rbrakk> \<Longrightarrow> P"
+lemma consis_join_L_inv[elim!]: "\<lbrakk> v1\<sqinter>v2 ~ v; \<lbrakk> v1 ~ v; v2 ~ v \<rbrakk> \<Longrightarrow> P \<rbrakk> \<Longrightarrow> P"
   by auto
 
-lemma consis_join_R_inv[elim!]: "\<lbrakk> v ~ v1\<squnion>v2; \<lbrakk> v ~ v1; v ~ v2 \<rbrakk> \<Longrightarrow> P \<rbrakk> \<Longrightarrow> P"
+lemma consis_join_R_inv[elim!]: "\<lbrakk> v ~ v1\<sqinter>v2; \<lbrakk> v ~ v1; v ~ v2 \<rbrakk> \<Longrightarrow> P \<rbrakk> \<Longrightarrow> P"
   by (induction v arbitrary: v1 v2) auto
      
 lemma consis_sym_aux: "(v ~ v' \<longrightarrow> v' ~ v) \<and> (\<not> v ~ v' \<longrightarrow> \<not> v' ~ v)"
@@ -63,7 +63,7 @@ corollary consis_upper_bound: fixes v1::val and v2::val
   assumes v1_v2: "v1 ~ v2" and v_v1: "is_val v1" and v_v2: "is_val v2"
   shows "\<exists> v3. v1 \<sqsubseteq> v3 \<and> v2 \<sqsubseteq> v3 \<and> is_val v3"
 proof -
-  obtain v12 where v12: "v1 \<squnion> v2 = Some v12" and v_v12: "is_val v12" 
+  obtain v12 where v12: "v1 \<sqinter> v2 = Some v12" and v_v12: "is_val v12" 
     using v1_v2 v_v1 v_v2 consis_join_val by blast
   have 1: "v1 \<sqsubseteq> v12" using v12 le_join_left by blast
   have 2: "v2 \<sqsubseteq> v12" using v12 le_join_right by blast
@@ -85,7 +85,7 @@ lemma upper_bound_consis: fixes v1::val and v2::val and v3::val
     
 
   
-lemma d_consis_nat_L: "\<lbrakk> \<Gamma> \<turnstile> c : v; \<Gamma> = [VNat n] \<rbrakk> \<Longrightarrow> v ~ VNat n"
+lemma d_consis_nat_L: "\<lbrakk> \<Gamma> \<turnstile> c : v; \<Gamma> = [TNat n] \<rbrakk> \<Longrightarrow> v ~ TNat n"
   apply (induction \<Gamma> c v arbitrary: n rule: deduce_le.induct)
        apply (case_tac \<Gamma>1) apply force apply force
       apply (case_tac \<Gamma>1) apply force apply force
@@ -94,18 +94,18 @@ lemma d_consis_nat_L: "\<lbrakk> \<Gamma> \<turnstile> c : v; \<Gamma> = [VNat n
    apply force+
   done
 
-lemma le_any_nat_consis[intro]: "v \<sqsubseteq> VNat n \<Longrightarrow> v ~ VNat n"
-  unfolding le_val_def using d_consis_nat_L by auto
+lemma le_any_nat_consis[intro]: "TNat n <: v \<Longrightarrow> v ~ TNat n"
+  unfolding sub_ty_def using d_consis_nat_L by auto
 
-lemma consis_nat_atoms: "\<lbrakk> v ~ VNat n \<rbrakk> \<Longrightarrow> atoms v \<subseteq> { VNat n }"
+lemma consis_nat_atoms: "\<lbrakk> v ~ TNat n \<rbrakk> \<Longrightarrow> atoms v \<subseteq> { TNat n }"
   by (induction v arbitrary: n) auto
   
 (*
-lemma le_any_nat_atom_consis: "\<lbrakk> v \<sqsubseteq> VNat n \<rbrakk> \<Longrightarrow> atoms v \<subseteq> {VNat n}"
+lemma le_any_nat_atom_consis: "\<lbrakk> v \<sqsubseteq> TNat n \<rbrakk> \<Longrightarrow> atoms v \<subseteq> {TNat n}"
   using le_any_nat_inv_atoms by blast
 *)
 
-definition consis :: "val set \<Rightarrow> bool" where
+definition consis :: "ty set \<Rightarrow> bool" where
   "consis \<Gamma> \<equiv> (\<forall>v v'. v \<in> \<Gamma> \<longrightarrow> v' \<in> \<Gamma> \<longrightarrow> v ~ v')"
   
 lemma consis_atoms: "\<lbrakk> v1 ~ v2; v1' \<in> atoms v1; v2' \<in> atoms v2 \<rbrakk> \<Longrightarrow> v1' ~ v2'"
@@ -135,65 +135,66 @@ lemma val_consis_atoms: "is_val v \<Longrightarrow> consis (atoms v)"
   apply clarify using consis_sym consis_atoms apply blast
   done
   
-lemma consis_nat_trans: "\<lbrakk> v1 ~ VNat n; VNat n ~ v2 \<rbrakk> \<Longrightarrow> v1 ~ v2"
+lemma consis_nat_trans: "\<lbrakk> v1 ~ TNat n; TNat n ~ v2 \<rbrakk> \<Longrightarrow> v1 ~ v2"
   by (induction v1) auto   
 
-lemma consis_nat_trans2: "\<lbrakk> v1 ~ v2; v2 ~ VNat n \<rbrakk> \<Longrightarrow> v1 ~ VNat n"
+lemma consis_nat_trans2: "\<lbrakk> v1 ~ v2; v2 ~ TNat n \<rbrakk> \<Longrightarrow> v1 ~ TNat n"
   by (induction v2 arbitrary: v1 n) auto
 
-definition vals :: "val set \<Rightarrow> bool" where
+definition vals :: "ty set \<Rightarrow> bool" where
   "vals \<Gamma> \<equiv> (\<forall>v. v \<in> \<Gamma> \<longrightarrow> is_val v)"
   
-lemma nat_atom_consis_nat: "\<lbrakk>  VNat n \<in> atoms v; is_val v \<rbrakk> \<Longrightarrow> v ~ VNat n"
+lemma nat_atom_consis_nat: "\<lbrakk>  TNat n \<in> atoms v; is_val v \<rbrakk> \<Longrightarrow> v ~ TNat n"
   apply (induction v arbitrary: n)
     apply force
    apply force
   apply simp apply clarify apply (erule disjE) 
    apply (rule conjI) apply force
-    apply (subgoal_tac "v1 ~ VNat n") prefer 2 apply blast 
+    apply (subgoal_tac "v1 ~ TNat n") prefer 2 apply blast 
   using consis_nat_trans2 consis_sym apply blast
   apply (rule conjI) 
-   apply (subgoal_tac "v2 ~ VNat n") prefer 2 apply blast
+   apply (subgoal_tac "v2 ~ TNat n") prefer 2 apply blast
   using consis_nat_trans2 apply blast
   apply blast
   done    
   
-lemma le_nat_any_consis[intro!]: assumes n_v: "VNat n \<sqsubseteq> v" and v_v: "is_val v" 
-  shows "v ~ VNat n"
+lemma le_nat_any_consis[intro!]: assumes n_v: "v <: TNat n" and v_v: "is_val v" 
+  shows "v ~ TNat n"
 proof -
-  obtain c where "[v] \<turnstile> c : VNat n" using n_v unfolding le_val_def by blast
+  obtain c where "[v] \<turnstile> c : TNat n" using n_v unfolding sub_ty_def by blast
   then obtain v' where
-    vp_v: "v' \<in> (\<Union>v\<in>set [v]. atoms v)" and vp_n: "v' = VNat n"
+    vp_v: "v' \<in> (\<Union>v\<in>set [v]. atoms v)" and vp_n: "v' = TNat n"
     using d_nat_inv by presburger
-  have "VNat n \<in> atoms v" using vp_v vp_n by simp
-  with v_v show "v ~ VNat n" using nat_atom_consis_nat by blast
+  have "TNat n \<in> atoms v" using vp_v vp_n by simp
+  with v_v show "v ~ TNat n" using nat_atom_consis_nat by blast
 qed    
 
 lemma consis_le_inconsis_le:
-  "(v1' ~ v2' \<longrightarrow> (\<forall> v1 v2. v1 \<sqsubseteq> v1' \<and> v2 \<sqsubseteq> v2' \<longrightarrow> v1 ~ v2))
-  \<and> (\<not> v1' ~ v2' \<longrightarrow> (\<forall> v1 v2. v1' \<sqsubseteq> v1 \<and> v2' \<sqsubseteq> v2 \<longrightarrow> \<not> v1 ~ v2))"
+  "(v1' ~ v2' \<longrightarrow> (\<forall> v1 v2. v1' <: v1 \<and> v2' <: v2 \<longrightarrow> v1 ~ v2))
+  \<and> (\<not> v1' ~ v2' \<longrightarrow> (\<forall> v1 v2. v1 <: v1' \<and> v2 <: v2' \<longrightarrow> \<not> v1 ~ v2))"
   (is "?P v1' v2' \<and> ?Q v1' v2'")
 proof (induction v1' v2' rule: consistent.induct)
   case (1 n m)
   then show ?case apply (rule conjI) apply clarify 
-     apply (subgoal_tac "v1 ~ VNat n") prefer 2 using le_any_nat_consis apply auto[1]
-     apply (subgoal_tac "v2 ~ VNat n") prefer 2 using le_any_nat_consis apply auto[1]
+     apply (subgoal_tac "v1 ~ TNat n") prefer 2 using le_any_nat_consis apply auto[1]
+     apply (subgoal_tac "v2 ~ TNat n") prefer 2 using le_any_nat_consis apply auto[1]
     using consis_nat_trans consis_sym apply blast
     apply (rule impI) apply simp
-    using consis_atoms consistent.simps(1) le_nat_any_inv_atoms by blast
+    using consis_atoms consistent.simps(1) sub_nat_any_inv_atoms by blast
 next
   case (2 v1 v1' m)
   show ?case
   proof
-    show "?P (v1\<mapsto>v1') (VNat m)" by auto
+    show "?P (v1\<rightarrow>v1') (TNat m)" by auto
   next
-    show "?Q (v1\<mapsto>v1') (VNat m)"
+    show "?Q (v1\<rightarrow>v1') (TNat m)"
     proof clarify
-      fix v3 v4 assume "\<not> v1 \<mapsto> v1' ~ VNat m" and v11_v3: "v1 \<mapsto> v1' \<sqsubseteq> v3" and m_v4: "VNat m \<sqsubseteq> v4"
+      fix v3 v4 assume "\<not> v1 \<rightarrow> v1' ~ TNat m" and v11_v3: "v3 <: v1 \<rightarrow> v1'" and
+        m_v4: "v4 <: TNat m"
         and v3_v4: "v3 ~ v4"
-      have m_v4: "VNat m \<in> atoms v4" using m_v4 le_nat_any_inv_atoms by blast
-      obtain v2 v2' where v22_v3: "v2\<mapsto>v2' \<in> atoms v3" using v11_v3 le_fun_any_inv_atoms_ex by blast
-      have "\<not> (VNat m ~ v2\<mapsto>v2')" by simp
+      have m_v4: "TNat m \<in> atoms v4" using m_v4 sub_nat_any_inv_atoms by blast
+      obtain v2 v2' where v22_v3: "v2\<rightarrow>v2' \<in> atoms v3" using v11_v3 sub_fun_any_inv_atoms_ex by blast
+      have "\<not> (TNat m ~ v2\<rightarrow>v2')" by simp
       then have "\<not> (v4 ~ v3)" using v22_v3 m_v4 atoms_inconsis by blast
       then show False using v3_v4 using consis_sym by blast
     qed      
@@ -202,15 +203,15 @@ next
   case (3 n v2 v2')
   show ?case
   proof
-    show "?P (VNat n) (v2\<mapsto>v2')" by auto
+    show "?P (TNat n) (v2\<rightarrow>v2')" by auto
   next
-    show "?Q (VNat n) (v2\<mapsto>v2')"
+    show "?Q (TNat n) (v2\<rightarrow>v2')"
     proof clarify
-      fix v3 v4 assume "\<not> VNat n ~ (v2\<mapsto>v2')" and v11_v3: "v2 \<mapsto> v2' \<sqsubseteq> v4" and 
-        m_v4: "VNat n \<sqsubseteq> v3" and v3_v4: "v3 ~ v4"
-      have m_v4: "VNat n \<in> atoms v3" using m_v4 le_nat_any_inv_atoms by blast
-      obtain v1 v1' where v22_v3: "v1\<mapsto>v1' \<in> atoms v4" using v11_v3 le_fun_any_inv_atoms_ex by blast
-      have "\<not> (VNat n ~ v1\<mapsto>v1')" by simp
+      fix v3 v4 assume "\<not> TNat n ~ (v2\<rightarrow>v2')" and v11_v3: "v4 <: v2 \<rightarrow> v2'" and 
+        m_v4: "v3 <: TNat n" and v3_v4: "v3 ~ v4"
+      have m_v4: "TNat n \<in> atoms v3" using m_v4 sub_nat_any_inv_atoms by blast
+      obtain v1 v1' where v22_v3: "v1\<rightarrow>v1' \<in> atoms v4" using v11_v3 sub_fun_any_inv_atoms_ex by blast
+      have "\<not> (TNat n ~ v1\<rightarrow>v1')" by simp
       then have "\<not> (v3 ~ v4)" using v22_v3 m_v4 atoms_inconsis by blast
       then show False using v3_v4 using consis_sym by blast
     qed      
@@ -219,14 +220,14 @@ next
   case (4 v1 v1' v2 v2')
   show ?case
   proof
-    show "?P (v1\<mapsto>v1') (v2\<mapsto>v2')"
+    show "?P (v1\<rightarrow>v1') (v2\<rightarrow>v2')"
     proof clarify
-      fix v3 v4 assume v11_v22: "v1 \<mapsto> v1' ~ v2 \<mapsto> v2'" and v3_v11: "v3 \<sqsubseteq> v1\<mapsto>v1'" and 
-        v4_v22: "v4 \<sqsubseteq> v2\<mapsto>v2'" 
-      have v3_fun: "\<forall>v'. v' \<in> atoms v3 \<longrightarrow> (\<exists> A B. v' = A\<mapsto>B \<and> v1 \<sqsubseteq> A \<and> B \<sqsubseteq> v1')"
-        using v3_v11 using le_any_fun_inv_atoms by blast
-      have v4_fun: "\<forall>v'. v' \<in> atoms v4 \<longrightarrow> (\<exists> A B. v' = A\<mapsto>B \<and> v2 \<sqsubseteq> A \<and> B \<sqsubseteq> v2')"
-        using v4_v22 using le_any_fun_inv_atoms by blast          
+      fix v3 v4 assume v11_v22: "v1 \<rightarrow> v1' ~ v2 \<rightarrow> v2'" and v3_v11: "v1\<rightarrow>v1' <: v3" and 
+        v4_v22: "v2\<rightarrow>v2' <: v4" 
+      have v3_fun: "\<forall>v'. v' \<in> atoms v3 \<longrightarrow> (\<exists> A B. v' = A\<rightarrow>B \<and> A <: v1 \<and> v1' <: B)"
+        using v3_v11 using sub_any_fun_inv_atoms by blast
+      have v4_fun: "\<forall>v'. v' \<in> atoms v4 \<longrightarrow> (\<exists> A B. v' = A\<rightarrow>B \<and> A <: v2 \<and> v2' <: B)"
+        using v4_v22 using sub_any_fun_inv_atoms by blast          
       have "(v1 ~ v2 \<and> v1' ~ v2') \<or> \<not>(v1 ~ v2)" using v11_v22 by simp
       then show "v3 ~ v4"
       proof
@@ -234,9 +235,9 @@ next
         have "\<forall>a3 a4. a3 \<in> atoms v3 \<longrightarrow> a4 \<in> atoms v4 \<longrightarrow> a3 ~ a4"
         proof clarify
           fix a3 a4 assume a3_v3: "a3 \<in> atoms v3" and a4_v4: "a4 \<in> atoms v4"
-          obtain A3 B3 where a3: "a3=A3\<mapsto>B3" and v1_A3: "v1 \<sqsubseteq> A3" and B3_v1: "B3 \<sqsubseteq> v1'" 
+          obtain A3 B3 where a3: "a3=A3\<rightarrow>B3" and v1_A3: "A3 <: v1" and B3_v1: "v1' <: B3" 
             using v3_fun a3_v3 by blast
-          obtain A4 B4 where a4: "a4=A4\<mapsto>B4" and v2_A4: "v2 \<sqsubseteq> A4" and B4_v2: "B4 \<sqsubseteq> v2'" 
+          obtain A4 B4 where a4: "a4=A4\<rightarrow>B4" and v2_A4: "A4 <: v2" and B4_v2: "v2' <: B4" 
             using v4_fun a4_v4 by blast
           show "a3 ~ a4"
           proof (cases "A3 ~ A4")
@@ -254,9 +255,9 @@ next
         have "\<forall>a3 a4. a3 \<in> atoms v3 \<longrightarrow> a4 \<in> atoms v4 \<longrightarrow> a3 ~ a4"
         proof clarify
           fix a3 a4 assume a3_v3: "a3 \<in> atoms v3" and a4_v4: "a4 \<in> atoms v4"
-          obtain A3 B3 where a3: "a3=A3\<mapsto>B3" and v1_A3: "v1 \<sqsubseteq> A3" and B3_v1: "B3 \<sqsubseteq> v1'" 
+          obtain A3 B3 where a3: "a3=A3\<rightarrow>B3" and v1_A3: "A3 <: v1" and B3_v1: "v1' <: B3" 
             using v3_fun a3_v3 by blast
-          obtain A4 B4 where a4: "a4=A4\<mapsto>B4" and v2_A4: "v2 \<sqsubseteq> A4" and B4_v2: "B4 \<sqsubseteq> v2'" 
+          obtain A4 B4 where a4: "a4=A4\<rightarrow>B4" and v2_A4: "A4 <: v2" and B4_v2: "v2' <: B4" 
             using v4_fun a4_v4 by blast
           have "\<not> A3 ~ A4" using v1_v2 4 v1_A3 v2_A4 by blast
           then show "a3 ~ a4" using a3 a4 by simp              
@@ -265,14 +266,14 @@ next
       qed
     qed      
   next
-    show "?Q (v1\<mapsto>v1') (v2\<mapsto>v2')"
+    show "?Q (v1\<rightarrow>v1') (v2\<rightarrow>v2')"
     proof clarify
-      fix v3 v4 assume "\<not> v1 \<mapsto> v1' ~ v2 \<mapsto> v2'" and v11_v3: "v1 \<mapsto> v1' \<sqsubseteq> v3" and
-        v22_v4: "v2 \<mapsto> v2' \<sqsubseteq> v4" and v3_v4: "v3 ~ v4"
+      fix v3 v4 assume "\<not> v1 \<rightarrow> v1' ~ v2 \<rightarrow> v2'" and v11_v3: "v3 <: v1 \<rightarrow> v1'" and
+        v22_v4: "v4 <: v2 \<rightarrow> v2'" and v3_v4: "v3 ~ v4"
       then have v1_v2: "v1 ~ v2 \<and> \<not> v1' ~ v2'" by simp
-      obtain v31 v32 where v33_v3: "v31 \<mapsto> v32 \<in> atoms v3" 
-        using le_fun_any_inv_atoms_ex v11_v3 by blast
-      have "v31 \<sqsubseteq> v1 \<and> v1' \<sqsubseteq> v32" using v33_v3 v11_v3 le_fun_any_inv_atoms
+      obtain v31 v32 where v33_v3: "v31 \<rightarrow> v32 \<in> atoms v3" 
+        using sub_fun_any_inv_atoms_ex v11_v3 by blast
+      have "v1 <: v31 \<and> v32 <: v1'" using v33_v3 v11_v3 sub_fun_any_inv_atoms
         sorry    
           
       have "\<not> v3 ~ v4" sorry 
@@ -283,11 +284,11 @@ next
   case (5 n v2 v2')
   show ?case
   proof
-    show "?P (VNat n) (v2 \<squnion> v2')"   
-      by (metis consis_nat_atoms LaurentValues.le_trans atoms_le_any_nat consis_nat_trans 
+    show "?P (TNat n) (v2 \<sqinter> v2')"   
+      by (metis consis_nat_atoms sub_trans atoms_sub_any_nat consis_nat_trans 
           consis_sym le_any_nat_consis)
   next
-    show "?Q (VNat n) (v2 \<squnion> v2')" 
+    show "?Q (TNat n) (v2 \<sqinter> v2')" 
       sorry
   qed
 next
@@ -351,10 +352,10 @@ qed
   done
 *)
   
-lemma consis_le: "\<lbrakk> v1 \<sqsubseteq> v1'; v2 \<sqsubseteq> v2'; v1' ~ v2' \<rbrakk> \<Longrightarrow> v1 ~ v2"
+lemma consis_le: "\<lbrakk> v1' <: v1; v2' <: v2; v1' ~ v2' \<rbrakk> \<Longrightarrow> v1 ~ v2"
   using consis_le_inconsis_le by blast
 
-lemma inconsis_le: "\<lbrakk> v1' \<sqsubseteq> v1; v2' \<sqsubseteq> v2; \<not> v1' ~ v2' \<rbrakk> \<Longrightarrow> \<not> v1 ~ v2"
+lemma inconsis_le: "\<lbrakk> v1 <: v1'; v2 <: v2'; \<not> v1' ~ v2' \<rbrakk> \<Longrightarrow> \<not> v1 ~ v2"
   using consis_le_inconsis_le by blast
     
 lemma lookup_consis[intro]: "\<lbrakk> consis_env \<rho> \<rho>'; x < length \<rho> \<rbrakk> \<Longrightarrow> (\<rho>!x) ~ (\<rho>'!x)"
@@ -366,17 +367,17 @@ lemma cons_val_env_inv[elim!]: "\<lbrakk> val_env (v#\<rho>); \<lbrakk> is_val v
 lemma ext_val_env[intro!]: "\<lbrakk> is_val v; val_env \<rho> \<rbrakk> \<Longrightarrow> val_env (v#\<rho>)"
    apply auto apply (case_tac k) apply auto done
 
-abbreviation join_env :: "val list \<Rightarrow> val list \<Rightarrow> val list" (infix "\<squnion>" 55) where
-  "\<rho> \<squnion> \<rho>' \<equiv> map (\<lambda>(v,v'). v \<squnion> v') (zip \<rho> \<rho>')"
+abbreviation join_env :: "ty list \<Rightarrow> ty list \<Rightarrow> ty list" (infix "\<sqinter>" 55) where
+  "\<rho> \<sqinter> \<rho>' \<equiv> map (\<lambda>(v,v'). v \<sqinter> v') (zip \<rho> \<rho>')"
     
-lemma consis_env_join: fixes \<rho>1::"val list" assumes r1_r2: "consis_env \<rho>1 \<rho>2" 
+lemma consis_env_join: fixes \<rho>1::"ty list" assumes r1_r2: "consis_env \<rho>1 \<rho>2" 
   and v_r1: "val_env \<rho>1" and v_r2: "val_env \<rho>2"
-  shows "val_env (\<rho>1 \<squnion> \<rho>2)" using r1_r2 v_r1 v_r2 by auto
+  shows "val_env (\<rho>1 \<sqinter> \<rho>2)" using r1_r2 v_r1 v_r2 by auto
     
 lemma consis_env_length: "consis_env \<rho> \<rho>' \<Longrightarrow> length \<rho> = length \<rho>'"
   by auto
 
-lemma join_env_length: "\<lbrakk> consis_env \<rho>1 \<rho>2 \<rbrakk> \<Longrightarrow> length (\<rho>1 \<squnion> \<rho>2) = length \<rho>1"
+lemma join_env_length: "\<lbrakk> consis_env \<rho>1 \<rho>2 \<rbrakk> \<Longrightarrow> length (\<rho>1 \<sqinter> \<rho>2) = length \<rho>1"
   by auto
          
 end
